posts/awful-user-experience-academic-research.md
@@ -33,9 +33,16 @@ long-windedness of the mathematical statements at stake.
 nope, because computers. in a tool with first-class metaprogramming, we can have both.
 
 also, because we can *locally* rename or alias symbols, we can have *explicit and local* terseness without requiring a globally useless name
-
+the length of a symbol's name should be inversely proportional to how often users will encounter that symbol. absolutely ubiquitous ones (`Theorem`, `forall`, `fun`, `Definition`) should have extremely terse or merely symbolic names. very uncommon ones should have very clear and descriptive names
 
 
 more than one name for the same thing
 there shouldn't be more than one way to do the same thing!
 if a syntax sugar exists for a more "flexible" version of something, then detect and require the sugar
+
+
+
+
+subset types can be better
+the `&` syntax puts props onto a type (in both logic and computation land) but it remains the base type you declared, just with more assertions. these extended types can be used for anything they can be coerced to (immediate or easily automated coercions don't require extra notation, more complex ones require some kind of `by _` or `by tactic` and then proving)
+proving theorems about a function using `function_name.thm` instead of bare `thm` (which implies only the return type? perhaps also about the arguments?) automatically puts the arguments of the function into context and implies the theorem is essentially adding a `&` subset type onto the result of that function. this can mean you can add props to an outside function if you import the module that includes your narrowing proof, it's like external impls
